<!-- 
licensed from Active Calculus MB development, https://github.com/mattboelkins/active-calculus-single-mbx/blob/doenet-embed/source/exercises/doenet/ez-1-3-doenet-3.xml
-->


<setup>

  <selectFromSequence assignNames="a" from="1.5" to="2.5" step="0.25" numToSelect="1"/>
  <selectFromSequence assignNames="b" from="0" to="2" step="0.5" numToSelect="1"/>  
  <selectFromSequence assignNames="c" from="-1.16" to="0.56" step="0.1" numToSelect="1"/> 

  <math name="ABSb"><abs>$b</abs></math>
  
  <function name="g" symbolic="false">-1*$a^x + $b</function>
  <derivative name="gP" symbolic="false">$g</derivative>  
  <function name="L" symbolic="false" styleNumber="3" labelPosition="lowerRight">$$gP($c)(x-$c) + $$g($c)</function>  
    <point name="A" styleNumber="2" coords="($c,$$g($c))" showCoordsWhenDragging="false" draggable="false" labelPosition="upperRight"> 
      <label><m>A = $A.coords</m></label>
    </point> 
    <point name="B" styleNumber="2" coords="($c+0.6*$a,$$L($c+0.6*$a))" showCoordsWhenDragging="false" draggable="false" labelPosition="upperRight"> 
      <label><m>B = $B.coords</m></label>
    </point>

  <label name="gLabel" anchor="(-3,$$g(-3)-0.25)"><m>y = g(x)</m></label>
  <label name="LLabel" anchor="(-3,$$L(-3)+0.25)"><m>y = L(x)</m></label>
  
</setup>

  <p>Let <m>g</m> be the function given by the graph below and <m>L</m> its tangent line at the point <m>A</m>.</p>

<!--  <p><m>a = $a</m>, <m>b = $b</m>, and <m>c = $c</m>, so <m>g(x) = $$g(x)</m> and <m>L(x) = $$L(x)</m>, plus <m>A = $A</m> and <m>B = $B</m></p> -->

    <figure>
      <graph xmin="-4" xmax="4" ymin="-4" ymax="4" size="medium" grid="false" showNavigation="false" displayXAxis="false" displayYAxis="false"> $g $L $A $B $gLabel $LLabel
      </graph>
      <caption>Plot of <m>y = g(x)</m> and its tangent line at the point <m>A</m></caption>
    </figure>

  <p>Use the given information to complete the following sentence. </p>  
  <p>At the point where <m>a = </m><answer><award allowedErrorInNumbers="0.01" allowedErrorIsAbsolute> $c
        </award></answer>, we know that <m>g(a) = </m><answer><award allowedErrorInNumbers="0.01" allowedErrorIsAbsolute> $$g($c)
        </award></answer> and <m>g'(a) = </m><answer><award allowedErrorInNumbers="0.01" allowedErrorIsAbsolute> $$gP($c)
        </award></answer>.</p>
   